func: Readability
There are no interesting code changes in this commit.

theories/lang/cpp/logic/func.v
@@ -24,363 +24,370 @@ Proof. iIntros "Q W R". iApply ("Q" with "(W R)"). Qed.
 
 #[local] Set Printing Coercions.
 
-Arguments ERROR {_ _} _%bs.
-Arguments UNSUPPORTED {_ _} _%bs.
+#[local] Arguments ERROR {_ _} _%bs.
+#[local] Arguments UNSUPPORTED {_ _} _%bs.
 #[local] Arguments wpi : simpl never.
 
-(** ** Weakest precondition of a constructor: Initial construction step.
-
-Makes [this] and immediate [members] of [cls] strictly valid, to implement the
-part of http://eel.is/c++draft/class.cdtor#3 about members.
-This enables their dereference via [wp_lval_deref].
+(** ** Weakest precondition of a constructor: Initial construction step. *)
+(**
+Makes [this] and immediate [members] of [cls] strictly valid, to
+implement the part of http://eel.is/c++draft/class.cdtor#3 about
+members. This enables their dereference via [wp_lval_deref].
 *)
-mlock Definition svalid_members `{Σ : cpp_logic thread_info} {resolve:genv}
-          (cls : globname)
-          (members : list (bs * type))
-          : Rep :=
+mlock Definition svalid_members `{Σ : cpp_logic, σ : genv}
+    (cls : globname) (members : list (bs * type)) : Rep :=
   reference_toR (Tnamed cls) **
-  [∗list] m ∈ members,
-    _field {| f_type := cls ; f_name := m.1 |} |-> reference_toR m.2.
+  [** list] m ∈ members,
+  _field {| f_type := cls ; f_name := m.1 |} |-> reference_toR m.2.
 #[global] Arguments svalid_members {_ _ _} _ _ : assert.
 
 Section svalid_members.
-  Context `{Σ : cpp_logic thread_info} {resolve:genv}.
+  Context `{Σ : cpp_logic, σ : genv}.
+
   #[global] Instance svalid_members_persistent : Persistent2 svalid_members.
-  Proof.
-    intros; rewrite svalid_members.unlock. refine _.
-  Qed.
+  Proof. rewrite svalid_members.unlock. apply _. Qed.
+
   #[global] Instance svalid_members_affine : Affine2 svalid_members := _.
 End svalid_members.
 
+(** ** Aggregate identity *)
+(**
+Part of [all_identities path cls], but indexed by fuel [f].
+
+TODO: Replace this with a version that is built by well-founded
+recursion.
+*)
+#[local]
+Definition derivationsR' `{Σ : cpp_logic, σ : genv} (tu : translation_unit) (q : cQp.t) :=
+  fix derivationsR' (f : nat) (include_base : bool) (cls : globname) (path : list globname) : Rep :=
+  match f with
+  | 0 => ERROR "derivationsR: no fuel"
+  | S f =>
+    match tu !! cls with
+    | Some (Gstruct st) =>
+      (if include_base && has_vtable st then derivationR cls path q else emp) **
+      [** list] b ∈ st.(s_bases),
+      let base := b.1 in
+      _base cls base |-> derivationsR' f true base (path ++ [base])
+    | _ => ERROR "derivationsR: not a structure"
+    end
+  end%I.
+
+(**
+[this |-> derivationsR include_base cls path q] is all of the object
+identities of the [this] object (of type [cls]) where the most derived
+class is reached from [cls] using [path]. For example, consider the
+following
+```c++
+class A {};
+class B : public A {};
+class C : public B {};
+```
+here, [derivationsR true "::B" ["::C"] q] produces:
+[[
+derivationR "::B" ["::C","::B"] q **
+_base "::B" "::A" |-> derivationR "::A" ["::C","::B","::A"] q
+]]
+
+while [derivationsR true "::C" [] q] produces all the identities for A, B and C:
+[[
+derivationR "::C" ["::C"] q **
+_base "::C" "::B" |-> derivationR true "::B" ["::C"] q
+]]
+*)
+Definition derivationsR `{Σ : cpp_logic, σ : genv} (tu : translation_unit)
+    (include_base : bool) (cls : globname) (path : list globname) (q : cQp.t) : Rep :=
+  (**
+  The number of global entries is an upper bound on the height of the
+  derivation tree.
+  *)
+  let size := avl.IM.cardinal σ.(genv_tu).(types) in
+  derivationsR' tu q size include_base cls path.
+
+(* conveniences for the common pattern *)
+Notation init_derivationR cls path q := (derivationR cls%bs (path%bs ++ [cls%bs]) q).
+Notation init_derivationsR cls path q := (derivationsR cls%bs (path%bs ++ [cls%bs]) q).
+
+(**
+[wp_init_identity cls Q] updates the identities of "this" by updating
+the [identity] of all base classes (transitively) and producing the
+new identity for "this".
+
+TODO: Make this an [mpred]
+*)
+Definition wp_init_identity `{Σ : cpp_logic, σ : genv} (tu : translation_unit)
+    (cls : globname) (Q : mpred) : Rep :=
+  derivationsR tu false cls [] (cQp.mut 1) **
+  (derivationsR tu true cls [cls] (cQp.mut 1) -* pureR Q).
+
 Section with_cpp.
-  Context `{Σ : cpp_logic thread_info} {resolve:genv}.
-  Variable tu : translation_unit.
+  Context `{Σ : cpp_logic, σ : genv}.
+  Implicit Types (p : ptr) (Q : mpred).
 
-  Notation wp := (wp tu).
-  Notation wpi := (wpi tu).
-  Notation wp_init := (wp_init tu).
-  #[local] Notation interp := (interp tu).
-
-  #[local] Open Scope free_scope.
-
-  #[local] Notation _base := (o_base resolve).
-  #[local] Notation _derived := (o_derived resolve).
-
-  Implicit Types p : ptr.
-
-  (** * Aggregate identity *)
-  (* Part of [all_identities path cls], but indexed by fuel [f].
-     TODO replace this with a version that is built by well-founded recursion.
-   *)
-  #[local]
-  Fixpoint derivationsR' (f : nat) (include_base : bool) (cls : globname) (path : list globname) (q : cQp.t) : Rep :=
-    match f with
-    | 0 => False
-    | S f =>
-      match tu !! cls with
-      | Some (Gstruct st) =>
-        (if include_base && has_vtable st then derivationR cls path q else emp) **
-        [∗list] b ∈ st.(s_bases),
-           let '(base,_) := b in
-           _base cls base |-> derivationsR' f true base (path ++ [base]) q
-      | _ => False
-      end
-    end.
-
-  (** [this |-> derivationsR include_base cls path q] is all of the object
-      identities of the [this] object (of type [cls]) where the most derived
-      class is reached from [cls] using [path]. For example, consider the
-      following
-      ```c++
-      class A {};
-      class B : public A {};
-      class C : public B {};
-      ```
-      here, [derivationsR true "::B" ["::C"] q] produces:
-      [[
-      derivationR "::B" ["::C","::B"] q **
-      _base "::B" "::A" |-> derivationR "::A" ["::C","::B","::A"] q
-      ]]
-
-      while [derivationsR true "::C" [] q] produces all the identities for A, B and C:
-      [[
-      derivationR "::C" ["::C"] q **
-      _base "::C" "::B" |-> derivationR true "::B" ["::C"] q
-      ]]
-   *)
-  Definition derivationsR : bool -> globname -> list globname -> cQp.t -> Rep :=
-    let size := avl.IM.cardinal resolve.(genv_tu).(types) in
-    (* ^ the number of global entries is an upper bound on the height of the
-       derivation tree.
-     *)
-    derivationsR' size.
-
-  (** [wp_init_identity cls Q] updates the identities of "this" by updating the
-      [identity] of all base classes (transitively) and producing the new identity
-      for "this".
-   *)
-  Definition wp_init_identity (cls : globname) (Q : mpred) : Rep :=
-    derivationsR false cls [] (cQp.mut 1) **
-    (derivationsR true cls [cls] (cQp.mut 1) -* pureR Q).
-
-  Theorem wp_init_identity_frame cls Q Q' :
-    pureR (Q' -* Q) |-- wp_init_identity cls Q' -* wp_init_identity cls Q.
+  Lemma wp_init_identity_frame tu cls Q Q' :
+    pureR (Q' -* Q) |-- wp_init_identity tu cls Q' -* wp_init_identity tu cls Q.
   Proof.
-    iIntros "X [$ Y] Z".
-    rewrite pureR_wand.
-    by iApply "X"; iApply "Y".
+    iIntros "X [$ Y] Z". rewrite pureR_wand. iApply "X". by iApply "Y".
   Qed.
 
-  (* variant of [wp_init_identity_frame] for [mpred]. *)
-  Theorem wp_init_identity_frame' cls Q Q' p :
-    Q' -* Q |-- (p |-> wp_init_identity cls Q') -* (p |-> wp_init_identity cls Q).
+  Lemma _at_wp_init_identity_frame tu cls Q Q' p :
+    Q' -* Q |-- (p |-> wp_init_identity tu cls Q') -* (p |-> wp_init_identity tu cls Q).
   Proof. by rewrite -_at_wand -wp_init_identity_frame _at_pureR. Qed.
+End with_cpp.
 
-  (** [wp_revert_identity cls Q] updates the identities of "this" by taking the
-      [identity] of this class and transitively updating the [identity] of all base
-      classes to remove [cls] as the most derived class.
-   *)
-  Definition wp_revert_identity (cls : globname) (Q : mpred) : Rep :=
-    derivationsR true cls [cls] (cQp.mut 1) **
-    (derivationsR false cls [] (cQp.mut 1) -* pureR Q).
+(**
+[wp_revert_identity cls Q] updates the identities of "this" by taking
+the [identity] of this class and transitively updating the [identity]
+of all base classes to remove [cls] as the most derived class.
 
-  Theorem wp_revert_identity_frame cls Q Q' :
-    pureR (Q' -* Q) |-- wp_revert_identity cls Q' -* wp_revert_identity cls Q.
+TODO: Make this an [mpred]
+*)
+Definition wp_revert_identity `{Σ : cpp_logic, σ : genv} (tu : translation_unit)
+    (cls : globname) (Q : mpred) : Rep :=
+  derivationsR tu true cls [cls] (cQp.mut 1) **
+  (derivationsR tu false cls [] (cQp.mut 1) -* pureR Q).
+
+Section with_cpp.
+  Context `{Σ : cpp_logic, σ : genv}.
+  Implicit Types (p : ptr) (Q : mpred).
+
+  Lemma wp_revert_identity_frame tu cls Q Q' :
+    pureR (Q' -* Q) |-- wp_revert_identity tu cls Q' -* wp_revert_identity tu cls Q.
   Proof.
-    iIntros "X [$ Y] Z".
-    rewrite pureR_wand.
-    by iApply "X"; iApply "Y".
+    iIntros "X [$ Y] Z". rewrite pureR_wand. iApply "X". by iApply "Y".
   Qed.
 
   (** sanity chect that initialization and revert are inverses *)
-  Corollary wp_init_revert cls Q p :
-    let REQ := derivationsR false cls [] (cQp.mut 1) in
-        p |-> REQ ** Q
-    |-- p |-> wp_init_identity cls (p |-> wp_revert_identity cls (p |-> REQ ** Q)).
+  Lemma wp_init_revert tu cls Q p :
+    let REQ := derivationsR tu false cls [] (cQp.mut 1) in
+    p |-> REQ ** Q
+    |-- p |-> wp_init_identity tu cls (p |-> wp_revert_identity tu cls (p |-> REQ ** Q)).
   Proof.
     rewrite /wp_revert_identity/wp_init_identity.
     rewrite !_at_sep !_at_wand !_at_pureR.
     iIntros "[$ $] $ $".
   Qed.
+End with_cpp.
+#[deprecated(since="20230820", note="use [_at_wp_init_identity_frame]")]
+Notation wp_init_identity_frame' := _at_wp_init_identity_frame (only parsing).
 
-  (** * Binding parameters *)
+(** ** Binding parameters *)
 
-  Fixpoint wp_make_mutables (ls : list (ptr * decltype)) (Q : epred) : mpred :=
-    match ls with
-    | nil => Q
-    | (p,t) :: ls => wp_make_mutables ls $ wp_make_mutable tu p t Q
-    end.
+Definition wp_make_mutables `{Σ : cpp_logic, σ : genv} (tu : translation_unit) :=
+  fix wp_make_mutables (args : list (ptr * decltype)) (Q : epred) : mpred :=
+  match args with
+  | nil => Q
+  | p :: args => wp_make_mutables args $ wp_make_mutable tu p.1 p.2 Q
+  end.
 
-  Lemma wp_make_mutables_frame ls : forall Q Q',
-      Q -* Q' |-- wp_make_mutables ls Q -* wp_make_mutables ls Q'.
+Section with_cpp.
+  Context `{Σ : cpp_logic, σ : genv}.
+  Implicit Types (Q : epred).
+
+  Lemma wp_make_mutables_frame tu args Q Q' :
+    Q -* Q' |-- wp_make_mutables tu args Q -* wp_make_mutables tu args Q'.
   Proof.
-    induction ls =>/=; eauto.
-    iIntros (??) "X"; case_match; iApply (IHls with "[X]").
-    iApply wp_const_frame; first reflexivity; eauto.
+    move: Q Q'. induction args; intros; first done. cbn. iIntros "HQ".
+    iApply (IHargs with "[HQ]"). by iApply wp_const_frame.
   Qed.
+End with_cpp.
 
-  Definition Kcleanup (ls : list (ptr * decltype)) : Kpred -> Kpred :=
-    Kat_exit (wp_make_mutables ls).
+Definition Kcleanup `{Σ : cpp_logic, σ : genv} (tu : translation_unit)
+    (args : list (ptr * decltype)) (Q : Kpred) : Kpred :=
+  Kat_exit (wp_make_mutables tu args) Q.
 
-  Lemma Kcleanup_frame ls (Q Q' : Kpred) rt :
-    Q rt -* Q' rt |-- Kcleanup ls Q rt -* Kcleanup ls Q' rt.
+Section with_cpp.
+  Context `{Σ : cpp_logic, σ : genv}.
+  Implicit Types (Q : Kpred).
+
+  Lemma Kcleanup_frame tu args (Q Q' : Kpred) rt :
+    Q rt -* Q' rt |-- Kcleanup tu args Q rt -* Kcleanup tu args Q' rt.
   Proof.
-    iIntros "K". iApply Kat_exit_frame; eauto.
-    iIntros (??) "X"; iApply wp_make_mutables_frame; eauto.
+    iIntros "?". iApply Kat_exit_frame; [|done].
+    iIntros (??) "?". by iApply wp_make_mutables_frame.
   Qed.
+End with_cpp.
 
-  (** [bind_vars args vals r Q] performs initialization of the parameters
-      given the values being passed.
+(**
+[bind_vars tu ar ts args ρ Q] initializes a function's arguments
+[args] according to its arity [ar] and declared parameter types [ts].
 
-      NOTE. We make arguments [const] here if necessary and then make them
-            mutable again in the second argument to [Q].
-   *)
-  Fixpoint bind_vars (args : list (ident * decltype)) (ar : function_arity) (ptrs : list ptr)
-    (ρ : option ptr -> region) (Q : region -> list (ptr * decltype) -> mpred) : mpred :=
-    match args with
-    | nil =>
-        match ar with
-        | Ar_Definite =>
-            match ptrs with
-            | nil => Q (ρ None) []
-            | _ :: _ => ERROR "bind_vars: extra arguments"
-            end
-        | Ar_Variadic =>
-            match ptrs with
-            | vap :: nil => Q (ρ $ Some vap) []
-            | _ => ERROR "bind_vars: variadic function missing varargs"
-            end
-        end
-    | (x,ty) :: xs =>
-        match ptrs with
-        | p :: ps =>
-            (*
-            NOTE: We need not gather additional qualifiers from an
-            array's element type as Clang's parser eagerly "decays" a
-            function's array parameter types to pointer types.
-            *)
-            let '(cv, ty) := decompose_type ty in
-            if q_const cv then
-              wp_make_const tu p ty $ bind_vars xs ar ps (fun vap => Rbind x p $ ρ vap)
-                (fun ρ consts => Q ρ $ (p,ty) :: consts)
-            else
-              bind_vars xs ar ps (fun vap => Rbind x p $ ρ vap) Q
-        | nil => ERROR "bind_vars: insufficient arguments"
-        end
-    end.
-
-
-  Lemma bind_vars_frame : forall ts ar args ρ Q Q',
-        Forall ρ free, Q ρ free -* Q' ρ free
-    |-- bind_vars ts ar args ρ Q -* bind_vars ts ar args ρ Q'.
-  Proof.
-    induction ts; destruct args => /= *; eauto.
-    { case_match; eauto.
-      iIntros "A B"; iApply "A"; eauto. }
-    { case_match; eauto. case_match; eauto.
-      iIntros "A"; iApply "A". }
-    { iIntros "A".
-      repeat case_match; subst.
-      { iApply wp_const_frame; first reflexivity.
-        iApply IHts. iIntros (??). iApply "A". }
-      { iApply IHts; iApply "A". } }
-  Qed.
-
-  (** * Weakest preconditions of the flavors of C++ "functions"  *)
-
-  (** ** the weakest precondition of a function *)
-  Definition wp_func (f : Func) (args : list ptr) (Q : ptr -> epred) : mpred :=
-    match f.(f_body) with
-    | None => False
-    | Some body =>
-      match body with
-      | Impl body =>
-        let ρ va := Remp None va f.(f_return) in
-        letI* ρ, cleanup := bind_vars f.(f_params) f.(f_arity) args ρ in
-        |> wp ρ body (Kcleanup cleanup $ Kreturn (funI x => |={⊤}=> |> Q x))
-      | Builtin builtin =>
-        wp_builtin_func builtin (Tfunction (cc:=f.(f_cc)) f.(f_return) (List.map snd f.(f_params))) args Q
-      end
-    end.
-
-  Definition func_ok (f : Func) (spec : function_spec)
-    : mpred :=
-      [| type_of_spec spec = type_of_value (Ofunction f) |] **
-      (* forall each argument, apply to [fs_spec] *)
-      □ Forall Q : ptr -> mpred, Forall vals,
-        spec.(fs_spec) vals Q -* wp_func f vals Q.
-
-  (** ** The weakest precondition of a method
-
-      Note that in the calling convention for methods, the [this] parameter
-      is passed directly rather than being materialized like normal parameters.
-   *)
-  Definition wp_method (m : Method) (args : list ptr)
-             (Q : ptr -> epred) : mpred :=
-    match m.(m_body) with
-    | None => False
-    | Some (UserDefined body) =>
+NOTE. We make arguments [const] here if necessary and then make them
+mutable again in the second argument to [Q].
+*)
+Definition bind_vars `{Σ : cpp_logic, σ : genv} (tu : translation_unit) (ar : function_arity) :=
+  fix bind_vars (ts : list (ident * decltype)) (args : list ptr)
+    (ρ : option ptr -> region) (Q : region -> list (ptr * decltype) -> epred) : mpred :=
+  match ts with
+  | nil =>
+    match ar with
+    | Ar_Definite =>
       match args with
-      | thisp :: rest_vals =>
-        let ρ va := Remp (Some thisp) va m.(m_return) in
-        letI* ρ, cleanup := bind_vars m.(m_params) m.(m_arity) rest_vals ρ in
-        |> wp ρ body (Kcleanup cleanup (Kreturn (funI x => |={⊤}=> |>Q x)))
-      | _ => False
+      | nil => Q (ρ None) []
+      | _ :: _ => ERROR "bind_vars: extra arguments"
       end
-    | Some _ => UNSUPPORTED "defaulted methods"%bs
-    end.
+    | Ar_Variadic =>
+      match args with
+      | vap :: nil => Q (ρ $ Some vap) []
+      | _ => ERROR "bind_vars: variadic function missing varargs"
+      end
+    end
+  | xty :: ts =>
+    match args with
+    | p :: args =>
+      (*
+      NOTE: We need not gather additional qualifiers from an array's
+      element type as Clang's parser eagerly "decays" a function's
+      array parameter types to pointer types.
+      *)
+      let recurse := bind_vars ts args (fun vap => Rbind xty.1 p $ ρ vap) in
+      let qty := decompose_type xty.2 in
+      let ty := qty.2 in
+      if q_const qty.1 then
+        let* := wp_make_const tu p ty in
+        let* ρ, consts := recurse in
+        Q ρ $ (p,ty) :: consts
+      else
+        recurse Q
+    | nil => ERROR "bind_vars: insufficient arguments"
+    end
+  end.
 
-  Definition method_ok (m : Method) (spec : function_spec)
-    : mpred :=
-    [| type_of_spec spec = type_of_value (Omethod m) |] **
-    (* forall each argument, apply to [fs_spec] *)
-    □ Forall Q : ptr -> mpred, Forall vals,
-      spec.(fs_spec) vals Q -* wp_method m vals Q.
+Section with_cpp.
+  Context `{Σ : cpp_logic, σ : genv}.
+  Implicit Types (Q : region -> list (ptr * decltype) -> epred).
 
-  (** ** Weakest precondition of a constructor *)
+  Lemma bind_vars_frame tu ar ts args ρ Q Q' :
+    Forall ρ free, Q ρ free -* Q' ρ free
+    |-- bind_vars tu ar ts args ρ Q -* bind_vars tu ar ts args ρ Q'.
+  Proof.
+    move: args ρ Q Q'. induction ts; intros [] *; cbn.
+    { destruct ar; eauto. iIntros "HQ ?". by iApply "HQ". }
+    { destruct ar; eauto. case_match; eauto. iIntros "HQ ?". by iApply "HQ". }
+    { eauto. }
+    { iIntros "HQ". case_match.
+      - iApply wp_const_frame; [done|]. iApply IHts. iIntros (??) "?". by iApply "HQ".
+      - iApply IHts. iIntros (??) "?". by iApply "HQ". }
+  Qed.
+End with_cpp.
 
-  (* initialization of members in the initializer list *)
-  Fixpoint wpi_members
-           (ρ : region) (cls : globname) (this : ptr)
-           (members : list Member) (inits : list Initializer)
-           (Q : mpred) : mpred :=
-    match members with
-    | nil => Q
-    | m :: members =>
-      match List.filter (fun i =>
-                           match i.(init_path) with
-                           | InitField x
-                           | InitIndirect ((x,_) :: _) _ => bool_decide (m.(mem_name) = x)
-                           | _ => false
-                           end) inits with
-      | nil =>
-        (* there is no initializer for this member, so we "default initialize" it
-           (see https://eel.is/c++draft/dcl.init#general-7 )
-         *)
+(** ** The weakest precondition of a function *)
+
+Definition wp_func `{Σ : cpp_logic, σ : genv} (tu : translation_unit)
+    (f : Func) (args : list ptr) (Q : ptr -> epred) : mpred :=
+  match f.(f_body) with
+  | None => ERROR "wp_func: no body"
+  | Some body =>
+    match body with
+    | Impl body =>
+      let ρ vap := Remp None vap f.(f_return) in
+      letI* ρ, cleanup := bind_vars tu f.(f_arity) f.(f_params) args ρ in
+      |> wp tu ρ body (Kcleanup tu cleanup $ Kreturn $ fun x => |={⊤}=> |> Q x)
+    | Builtin builtin =>
+      let ts := List.map snd f.(f_params) in
+      (**
+      TODO: This seems to ignore [f_arity].
+      *)
+      wp_builtin_func builtin (Tfunction (cc:=f.(f_cc)) f.(f_return) ts) args Q
+    end
+  end.
+
+Definition func_ok `{Σ : cpp_logic, σ : genv} (tu : translation_unit)
+    (f : Func) (spec : function_spec) : mpred :=
+  [| type_of_spec spec = type_of_value (Ofunction f) |] **
+  □ Forall (Q : ptr -> epred) vals,
+  spec.(fs_spec) vals Q -* wp_func tu f vals Q.
+
+(** ** The weakest precondition of a method *)
+(**
+Note that in the calling convention for methods, the [this] parameter
+is passed directly rather than being materialized like normal
+parameters.
+*)
+Definition wp_method `{Σ : cpp_logic, σ : genv} (tu : translation_unit)
+    (m : Method) (args : list ptr) (Q : ptr -> epred) : mpred :=
+  match m.(m_body) with
+  | None => ERROR "wp_method: no body"
+  | Some (UserDefined body) =>
+    match args with
+    | thisp :: rest_vals =>
+      let ρ va := Remp (Some thisp) va m.(m_return) in
+      letI* ρ, cleanup := bind_vars tu m.(m_arity) m.(m_params) rest_vals ρ in
+      |> wp tu ρ body (Kcleanup tu cleanup $ Kreturn $ fun x => |={⊤}=> |> Q x)
+    | _ => ERROR "wp_method: no arguments"
+    end
+  | Some _ => UNSUPPORTED "wp_method: defaulted methods"
+  end.
+
+Definition method_ok `{Σ : cpp_logic, σ : genv} (tu : translation_unit)
+    (m : Method) (spec : function_spec) : mpred :=
+  [| type_of_spec spec = type_of_value (Omethod m) |] **
+  □ Forall (Q : ptr -> mpred) vals,
+  spec.(fs_spec) vals Q -* wp_method tu m vals Q.
+
+(** ** Weakest precondition of a constructor *)
+
+(**
+Initialization of members in the initializer list
+*)
+Definition wpi_members `{Σ : cpp_logic, σ : genv} (tu : translation_unit) (ρ : region)
+    (cls : globname) (this : ptr) (inits : list Initializer) :=
+  fix wpi_members (members : list Member) (Q : epred) : mpred :=
+  match members with
+  | nil => Q
+  | m :: members =>
+    let initializer_for (i : Initializer) :=
+      match i.(init_path) with
+      | InitField x
+      | InitIndirect ((x,_) :: _) _ => bool_decide (m.(mem_name) = x)
+      | _ => false
+      end
+    in
+    match List.filter initializer_for inits with
+    | nil =>
+      (*
+      there is no initializer for this member, so we "default
+      initialize" it (see https://eel.is/c++draft/dcl.init#general-7 )
+      *)
+      let* frees :=
         default_initialize tu m.(mem_type)
           (this ,, _field {| f_type := cls ; f_name := m.(mem_name) |})
-          (fun frees => interp frees (wpi_members ρ cls this members inits Q))
-      | i :: is' =>
-        match i.(init_path) with
-        | InitField _ (* = m.(mem_name) *) =>
-          match is' with
-          | nil =>
-            (* there is a *unique* initializer for this field *)
-            wpi ρ cls this i (wpi_members ρ cls this members inits Q)
-          | _ =>
-            (* there are multiple initializers for this field *)
-            ERROR $ "multiple initializers for field: " ++ cls ++ "::" ++ m.(mem_name)
-          end
-        | InitIndirect _ _ =>
-          (* this is initializing an object via sub-objets using indirect initialization.
-             TODO currently not supported
-           *)
-          UNSUPPORTED $ "indirect initialization: " ++ cls ++ "::" ++ m.(mem_name)
-        | _ => False (* unreachable due to the filter *)
+      in
+      let* := interp tu frees in
+      wpi_members members Q
+    | i :: is' =>
+      match i.(init_path) with
+      | InitField _ (* = m.(mem_name) *) =>
+        match is' with
+        | nil =>
+          (* there is a *unique* initializer for this field *)
+          wpi tu ρ cls this i (wpi_members members Q)
+        | _ =>
+          (* there are multiple initializers for this field *)
+          ERROR ("multiple initializers for field: " ++ cls ++ "::" ++ m.(mem_name))
         end
+      | InitIndirect _ _ =>
+        (*
+        this is initializing an object via sub-objets using indirect
+        initialization.
+
+        TODO currently not supported
+        *)
+        UNSUPPORTED ("indirect initialization: " ++ cls ++ "::" ++ m.(mem_name))
+      | _ => False%I (* unreachable due to the filter *)
       end
-    end%I%bs.
+    end
+  end.
 
-  (* initialization of bases in the initializer list *)
-  Fixpoint wpi_bases (ρ : region) (cls : globname) (this : ptr)
-           (bases : list globname) (inits : list Initializer)
-           (Q : mpred) : mpred :=
-    match bases with
-    | nil => Q
-    | b :: bases =>
-      match List.filter (fun i => bool_decide (i.(init_path) = InitBase b)) inits with
-      | nil =>
-        (* there is no initializer for this base class, so we use the default constructor *)
-        ERROR $ "missing base class initializer: " ++ cls
-      | i :: nil =>
-        (* there is an initializer for this class *)
-        wpi ρ cls this i (wpi_bases ρ cls this bases inits Q)
-      | _ :: _ :: _ =>
-        (* there are multiple initializers for this, so we fail *)
-        ERROR $ "multiple initializers for base: " ++ cls ++ "::" ++ b
-      end
-    end%I%bs.
+Section with_cpp.
+  Context `{Σ : cpp_logic, σ : genv}.
+  Implicit Types (p : ptr) (Q : epred).
 
-  Lemma wpi_bases_frame:
-    ∀ ρ p (ty : globname) bases (inits : list Initializer) (Q Q' : mpredI),
-      Q -* Q'
-      |-- wpi_bases ρ ty p bases inits Q -* wpi_bases ρ ty p bases inits Q'.
+  Lemma wpi_members_frame tu ρ cls this inits flds Q Q' :
+    Q -* Q'
+    |-- wpi_members tu ρ cls this inits flds Q -* wpi_members tu ρ cls this inits flds Q'.
   Proof.
-    induction bases => /=; eauto.
-    intros.
-    case_match; eauto.
-    case_match; eauto.
-    iIntros "a".
-    iApply wpi_frame => //.
-    by iApply IHbases.
-  Qed.
-
-  Lemma wpi_members_frame:
-    ∀ (ρ : region) flds p (ty : globname) (li : list Initializer) (Q Q' : mpredI),
-      Q -* Q'
-      |-- wpi_members ρ ty p flds li Q -* wpi_members ρ ty p flds li Q'.
-  Proof.
-    induction flds => /=; eauto; intros.
+    move: Q Q'. induction flds; intros; first done. cbn.
     case_match.
     { iIntros "a"; iApply default_initialize_frame; [done|].
       iIntros (?); iApply interp_frame. by iApply IHflds. }
@@ -390,42 +397,96 @@ Section with_cpp.
       iApply wpi_frame => //.
       by iApply IHflds. }
   Qed.
+End with_cpp.
 
-  Definition wp_struct_initializer_list (s : Struct) (ρ : region) (cls : globname) (this : ptr)
-             (inits : list Initializer) (Q : mpred) : mpred :=
-    match List.find (fun i => bool_decide (i.(init_path) = InitThis)) inits with
-    | Some {| init_type := ty ; init_init := e |} =>
-      match inits with
-      | _ :: nil =>
-        if bool_decide (drop_qualifiers ty = Tnamed cls) then
-          (* this is a delegating constructor, simply delegate. *)
-          wp_init ρ (Tnamed cls) this e (fun frees => interp frees Q)
-        else
-          (* the type names do not match, this should never happen *)
-          ERROR "type name mismatch"
-      | _ =>
-        (* delegating constructors are not allowed to have any other initializers
-         *)
-        ERROR "delegating constructor has other initializers"
-      end
-    | None =>
-      let bases := wpi_bases ρ cls this (List.map fst s.(s_bases)) inits in
-      let members := wpi_members ρ cls this s.(s_fields) inits in
-      let ident Q := this |-> wp_init_identity cls Q in
-      (** Provide strict validity for [this] and immediate members,
-      initialize the bases, then the identity, then initialize the members, following
-      http://eel.is/c++draft/class.base.init#13 (except virtual base classes, which are unsupported) *)
-      this |-> svalid_members cls ((fun m => (m.(mem_name), m.(mem_type))) <$> s.(s_fields)) -*
-      bases (ident (members (this |-> structR cls (cQp.mut 1) -* Q)))
-      (* NOTE we get the [structR] at the end since
-         [structR (cQp.mut 1) cls |-- type_ptrR (Tnamed cls)].
-       *)
-    end.
+(**
+Initialization of bases in the initializer list
+*)
+Definition wpi_bases `{Σ : cpp_logic, σ : genv} (tu : translation_unit)
+    (ρ : region) (cls : globname) (this : ptr) (inits : list Initializer) :=
+  fix wpi_bases (bases : list globname) (Q : epred) : mpred :=
+  match bases with
+  | nil => Q
+  | b :: bases =>
+    match List.filter (fun i => bool_decide (i.(init_path) = InitBase b)) inits with
+    | nil =>
+      (*
+      There is no initializer for this base class.
 
-  Lemma wp_struct_initializer_list_frame : forall ρ cls p ty li Q Q',
-      Q -* Q' |-- wp_struct_initializer_list cls ρ ty p li Q -* wp_struct_initializer_list cls ρ ty p li Q'.
+      TODO: Use the default constructor, or drop this TODO
+      *)
+      ERROR ("missing base class initializer: " ++ cls)
+    | i :: nil =>
+      (* there is an initializer for this class *)
+      wpi tu ρ cls this i (wpi_bases bases Q)
+    | _ :: _ :: _ =>
+      (* there are multiple initializers for this, so we fail *)
+      ERROR ("multiple initializers for base: " ++ cls ++ "::" ++ b)
+    end
+  end.
+
+Section with_cpp.
+  Context `{Σ : cpp_logic, σ : genv}.
+  Implicit Types (p : ptr) (Q : epred).
+
+  Lemma wpi_bases_frame tu ρ cls p inits bases Q Q' :
+    Q -* Q'
+    |-- wpi_bases tu ρ cls p inits bases Q -* wpi_bases tu ρ cls p inits bases Q'.
   Proof.
-    rewrite /wp_struct_initializer_list/=. intros. case_match.
+    move: Q Q'. induction bases; intros; first done. cbn.
+    case_match; eauto.
+    case_match; eauto.
+    iIntros "a".
+    iApply wpi_frame => //.
+    by iApply IHbases.
+  Qed.
+End with_cpp.
+
+Definition wp_struct_initializer_list `{Σ : cpp_logic, σ : genv} (tu : translation_unit)
+    (s : Struct) (ρ : region) (cls : globname) (this : ptr)
+    (inits : list Initializer) (Q : epred) : mpred :=
+  match List.find (fun i => bool_decide (i.(init_path) = InitThis)) inits with
+  | Some {| init_type := ty ; init_init := e |} =>
+    match inits with
+    | _ :: nil =>
+      if bool_decide (drop_qualifiers ty = Tnamed cls) then
+        (* this is a delegating constructor, simply delegate. *)
+        wp_init tu ρ (Tnamed cls) this e (fun frees => interp tu frees Q)
+      else
+        (* the type names do not match, this should never happen *)
+        ERROR "type name mismatch"
+    | _ =>
+      (*
+      delegating constructors are not allowed to have any other
+      initializers
+      *)
+      ERROR "delegating constructor has other initializers"
+    end
+  | None =>
+    let bases := wpi_bases tu ρ cls this inits (List.map fst s.(s_bases)) in
+    let members := wpi_members tu ρ cls this inits s.(s_fields) in
+    let ident Q := this |-> wp_init_identity tu cls Q in
+    (**
+    Provide strict validity for [this] and immediate members,
+    initialize the bases, then the identity, then initialize the
+    members, following http://eel.is/c++draft/class.base.init#13
+    (except virtual base classes, which are unsupported)
+
+    NOTE we get the [structR] at the end since [structR (cQp.mut 1)
+    cls |-- type_ptrR (Tnamed cls)].
+    *)
+    this |-> svalid_members cls ((fun m => (m.(mem_name), m.(mem_type))) <$> s.(s_fields)) -*
+    bases (ident (members (this |-> structR cls (cQp.mut 1) -* Q)))
+  end.
+Section with_cpp.
+  Context `{Σ : cpp_logic, σ : genv}.
+  Implicit Types (p : ptr) (Q : epred).
+
+  Lemma wp_struct_initializer_list_frame tu s ρ cls p inits Q Q' :
+    Q -* Q'
+    |-- wp_struct_initializer_list tu s ρ cls p inits Q -* wp_struct_initializer_list tu s ρ cls p inits Q'.
+  Proof.
+    rewrite /wp_struct_initializer_list/=. case_match.
     { case_match => //.
       destruct l; eauto.
       case_match; eauto.
@@ -435,229 +496,279 @@ Section with_cpp.
     { iIntros "Q".
       iApply wand_frame.
       iApply wpi_bases_frame.
-      iApply wp_init_identity_frame'.
+      iApply _at_wp_init_identity_frame.
       iApply wpi_members_frame.
       by iApply wand_frame. }
   Qed.
+End with_cpp.
 
-  Definition wp_union_initializer_list (u : translation_unit.Union) (ρ : region) (cls : globname) (this : ptr)
-             (inits : list Initializer) (Q : mpred) : mpred :=
-    match inits with
-    | [] => Q
-    | [{| init_path := InitField f ; init_type := te ; init_init := e |} as init] =>
-        match list_find (fun m => f = m.(mem_name)) u.(u_fields) with
-        | None => ERROR "field not found in union initialization"
-        | Some (n, m) => wpi ρ cls this init $ this |-> unionR cls (cQp.m 1) (Some n) -* Q
-        end
-    | _ =>
-      UNSUPPORTED "indirect (or self) union initialization is not currently supported"
-    end.
+Definition wp_union_initializer_list `{Σ : cpp_logic, σ : genv} (tu : translation_unit)
+    (u : translation_unit.Union) (ρ : region) (cls : globname) (this : ptr)
+    (inits : list Initializer) (Q : epred) : mpred :=
+  match inits with
+  | [] => Q
+  | [{| init_path := InitField f ; init_type := te ; init_init := e |} as init] =>
+    match list_find (fun m => f = m.(mem_name)) u.(u_fields) with
+    | None => ERROR "field not found in union initialization"
+    | Some (n, m) => wpi tu ρ cls this init $ this |-> unionR cls (cQp.m 1) (Some n) -* Q
+    end
+  | _ =>
+    UNSUPPORTED "indirect (or self) union initialization is not currently supported"
+  end.
 
-  Lemma wp_union_initializer_list_frame : forall ρ cls p ty li (Q Q' : epred),
-        (Q -* Q')
-    |-- wp_union_initializer_list cls ρ ty p li Q -*
-        wp_union_initializer_list cls ρ ty p li Q'.
+Section with_cpp.
+  Context `{Σ : cpp_logic, σ : genv}.
+  Implicit Types (p : ptr) (Q : epred).
+
+  Lemma wp_union_initializer_list_frame tu u ρ cls p inits Q Q' :
+    Q -* Q'
+    |-- wp_union_initializer_list tu u ρ cls p inits Q -* wp_union_initializer_list tu u ρ cls p inits Q'.
   Proof.
-    rewrite /wp_union_initializer_list/=. intros. case_match; eauto.
+    rewrite /wp_union_initializer_list/=. case_match; eauto.
     { iIntros "K".
       repeat case_match; eauto.
       iApply wpi_frame; [done|].
       iIntros "X Y"; iApply "K"; iApply "X"; done. }
   Qed.
+End with_cpp.
 
-  (** A special version of return to match the C++ rule that
-     constructors and destructors must not syntactically return a value, e.g.
-     `return f()` for `void f()` are not allowed.
+(**
+A special version of return to match the C++ rule that constructors
+and destructors must not syntactically return a value, e.g. `return
+f()` for `void f()` are not allowed.
 
-     NOTE: we could drop this in favor of relying on the compiler to
-           check this.
-   *)
-  Definition Kreturn_void (P : mpred) : KpredI :=
-    KP (funI rt =>
-          match rt with
-          | Normal | ReturnVoid => P
-          | _ => False
-          end).
+NOTE: we could drop this in favor of relying on the compiler to check
+this.
+*)
+Definition Kreturn_void `{Σ : cpp_logic} (P : mpred) : Kpred :=
+  KP $ funI rt =>
+  match rt with
+  | Normal | ReturnVoid => P
+  | _ => False
+  end.
 
-  (**
-     [wp_ctor ctor args Q] is the weakest pre-condition (with post-condition [Q])
-     running the constructor [ctor] with arguments [args].
+(**
+[wp_ctor tu ctor args Q] is the weakest pre-condition (with
+post-condition [Q]) running the constructor [ctor] with arguments
+[args].
 
-     Note that the constructor semantics consumes the entire [blockR] of the object
-     that is being constructed and the C++ abstract machine breaks this block down
-     producing usable† memory.
-     **Alternative**: Because constructor calls are *always* syntactically distinguished
-     (since C++ does not allow taking a pointer to a constructor), we know that any
-     invocation of a constructor will be from a [wp_init] which means that the C++
-     abstract machine will already own the memory (see the documentation for [wp_init]
-     in [wp.v]). In order to enforce this semantically within the abstract machine,
-     we would need a new predicate to say "a constructor with the given specification"
-     (rather than simply desugaring this to "a function with the given specification").
+Note that the constructor semantics consumes the entire [blockR] of
+the object that is being constructed and the C++ abstract machine
+breaks this block down producing usable† memory.
 
-     NOTE: supporting virtual inheritence will require us to add
-     constructor kinds here
+**Alternative**: Because constructor calls are *always* syntactically
+distinguished (since C++ does not allow taking a pointer to a
+constructor), we know that any invocation of a constructor will be
+from a [wp_init] which means that the C++ abstract machine will
+already own the memory (see the documentation for [wp_init] in
+[wp.v]). In order to enforce this semantically within the abstract
+machine, we would need a new predicate to say "a constructor with the
+given specification" (rather than simply desugaring this to "a
+function with the given specification").
 
-     † It is not necessarily initialized, e.g. because primitive fields are not
-       initialized (you get an [uninitR]), but you will get something that implies
-       [type_ptr].
-   *)
-  Definition wp_ctor (ctor : Ctor) (args : list ptr) (Q : ptr -> epred) : mpred :=
-    match ctor.(c_body) with
-    | None => False
-    | Some Defaulted => UNSUPPORTED "defaulted constructors"
-      (* ^ defaulted constructors are not supported yet *)
-    | Some (UserDefined (inits, body)) =>
-      match args with
-      | thisp :: rest_vals =>
-        let ty := Tnamed ctor.(c_class) in
-        match tu !! ctor.(c_class) with
-        | Some (Gstruct cls) =>
-          (* this is a structure *)
-          thisp |-> tblockR ty (cQp.mut 1) **
-          (* ^ this requires that you give up the *entire* block of memory that the object
-             will use.
-           *)
-          |> let ρ va := Remp (Some thisp) va Tvoid in
-             bind_vars ctor.(c_params) ctor.(c_arity) rest_vals ρ (fun ρ cleanup =>
-               (wp_struct_initializer_list cls ρ ctor.(c_class) thisp inits
-                  (wp ρ body (Kcleanup cleanup (Kreturn_void (|={⊤}=> |> Forall p : ptr, p |-> primR Tvoid (cQp.mut 1) Vvoid -* Q p))))))
-        | Some (Gunion union) =>
-        (* this is a union *)
-          thisp |-> tblockR ty (cQp.mut 1) **
-          (* ^ this requires that you give up the *entire* block of memory that the object
-             will use.
-           *)
-          |> let ρ va := Remp (Some thisp) va Tvoid in
-             bind_vars ctor.(c_params) ctor.(c_arity) rest_vals ρ (fun ρ cleanup =>
-               (wp_union_initializer_list union ρ ctor.(c_class) thisp inits
-                  (wp ρ body (Kcleanup cleanup (Kreturn_void (|={⊤}=> |> Forall p, p |-> primR Tvoid (cQp.mut 1) Vvoid -* Q p))))))
-        | _ =>
-            ERROR $ "constructor for non-aggregate (" ++ ctor.(c_class) ++ ")"
+NOTE: supporting virtual inheritence will require us to add
+constructor kinds here
+
+† It is not necessarily initialized, e.g. because primitive fields are
+not initialized (you get an [uninitR]), but you will get something
+that implies [type_ptr].
+*)
+Definition wp_ctor `{Σ : cpp_logic, σ : genv} (tu : translation_unit)
+    (ctor : Ctor) (args : list ptr) (Q : ptr -> epred) : mpred :=
+  match ctor.(c_body) with
+  | None => ERROR "wp_ctor: no body"
+  | Some Defaulted => UNSUPPORTED "defaulted constructors"
+  | Some (UserDefined (inits, body)) =>
+    match args with
+    | thisp :: rest_vals =>
+      let ty := Tnamed ctor.(c_class) in
+      match tu !! ctor.(c_class) with
+      | Some (Gstruct cls) =>
+        (*
+        this is a structure.
+
+        We require that you give up the *entire* block of memory
+        [tblockR] that the object will use.
+        *)
+        thisp |-> tblockR ty (cQp.mut 1) **
+        |>
+        let ρ vap := Remp (Some thisp) vap Tvoid in
+        let* ρ, cleanup := bind_vars tu ctor.(c_arity) ctor.(c_params) rest_vals ρ in
+        let* := wp_struct_initializer_list tu cls ρ ctor.(c_class) thisp inits in
+        let* := wp tu ρ body in
+        let* := Kcleanup tu cleanup in
+        let* := Kreturn_void in
+        |={⊤}=> |>
+        Forall p : ptr, p |-> primR Tvoid (cQp.mut 1) Vvoid -* Q p
+
+      | Some (Gunion union) =>
+        (*
+        this is a union.
+
+        We require that you give up the *entire* block of memory
+        [tblockR] that the object will use.
+        *)
+        thisp |-> tblockR ty (cQp.mut 1) **
+        |>
+        let ρ vap := Remp (Some thisp) vap Tvoid in
+        let* ρ, cleanup := bind_vars tu ctor.(c_arity) ctor.(c_params) rest_vals ρ in
+        let* := wp_union_initializer_list tu union ρ ctor.(c_class) thisp inits in
+        let* := wp tu ρ body in
+        let* := Kcleanup tu cleanup in
+        let* := Kreturn_void in
+        |={⊤}=> |>
+        Forall p : ptr, p |-> primR Tvoid (cQp.mut 1) Vvoid -* Q p
+
+      | _ => ERROR ("constructor for non-aggregate (" ++ ctor.(c_class) ++ ")")
+      end
+    | _ => ERROR "constructor without leading [this] argument"
+    end
+  end%I.
+
+Definition ctor_ok `{Σ : cpp_logic, σ : genv} (tu : translation_unit)
+    (ctor : Ctor) (spec : function_spec) : mpred :=
+  [| type_of_spec spec = type_of_value (Oconstructor ctor) |] **
+  □ Forall (Q : ptr -> epred) vals,
+  spec.(fs_spec) vals Q -* wp_ctor tu ctor vals Q.
+
+
+(** ** Weakest precondition of a destructor *)
+
+Definition wpd_bases `{Σ : cpp_logic, σ : genv} (tu : translation_unit)
+    (cls : globname) (this : ptr) (bases : list globname) (Q : epred) : mpred :=
+  let del_base base := FreeTemps.delete (Tnamed base) (this ,, _base cls base) in
+  interp tu (FreeTemps.seqs_rev (List.map del_base bases)) Q.
+
+Section with_cpp.
+  Context `{Σ : cpp_logic, σ : genv}.
+  Implicit Types (Q : epred).
+
+  Lemma wpd_bases_frame tu cls this bases Q Q' :
+    Q -* Q' |-- wpd_bases tu cls this bases Q -* wpd_bases tu cls this bases Q'.
+  Proof. apply interp_frame. Qed.
+End with_cpp.
+
+Definition wpd_members `{Σ : cpp_logic, σ : genv} (tu : translation_unit)
+    (cls : globname) (this : ptr) (members : list Member) (Q : epred) : mpred :=
+  let del_member m := FreeTemps.delete m.(mem_type) (this ,, _field {| f_name := m.(mem_name) ; f_type := cls |}) in
+  interp tu (FreeTemps.seqs_rev (List.map del_member members)) Q.
+
+Section with_cpp.
+  Context `{Σ : cpp_logic, σ : genv}.
+  Implicit Types (Q : epred).
+
+  Lemma wpd_members_frame tu cls this members Q Q' :
+    Q -* Q' |-- wpd_members tu cls this members Q -* wpd_members tu cls this members Q'.
+  Proof. apply interp_frame. Qed.
+End with_cpp.
+
+(**
+[wp_dtor tu dtor args Q] defines the semantics of the destructor
+[dtor] when applied to [args] with post-condition [Q].
+
+Note that destructors are not always syntactically distinguished from
+function calls (e.g. in the case of [c.~C()]). Therefore, in order to
+have a uniform specification, they need to return the underlying
+memory (i.e. a [this |-> tblockR (Tnamed cls) 1]) to the caller. When
+the program is destroying this object, e.g. due to stack allocation,
+this resource will be consumed immediately.
+*)
+Definition wp_dtor `{Σ : cpp_logic, σ : genv} (tu : translation_unit)
+    (dtor : Dtor) (args : list ptr) (Q : ptr -> epred) : mpred :=
+  match dtor.(d_body) with
+  | None => ERROR "wp_dtor: no body"
+  | Some body =>
+    let epilog :=
+      match tu !! dtor.(d_class) with
+      | Some (Gstruct s) => Some $ fun (thisp : ptr) =>
+        thisp |-> structR dtor.(d_class) (cQp.mut 1) **
+        (** Destroy fields *)
+        let* := wpd_members tu dtor.(d_class) thisp s.(s_fields) in
+        (** Destroy identity of the object *)
+        thisp |-> wp_revert_identity tu dtor.(d_class) (
+          (** Destroy base classes (reverse order) *)
+          let* := wpd_bases tu dtor.(d_class) thisp (List.map fst s.(s_bases)) in
+          (**
+          Destroy each object returning its memory to the abstract
+          machine. Then the abstract machine gives this memory back to
+          the program.
+
+          NOTE the [|>] here is for the function epilog.
+          *)
+          thisp |-> tblockR (Tnamed dtor.(d_class)) (cQp.mut 1) -*
+          |={⊤}=> |> Forall p : ptr, p |-> primR Tvoid (cQp.mut 1) Vvoid -* Q p
+        )
+      | Some (Gunion u) => Some $ fun (thisp : ptr) =>
+        (*
+        the function epilog of a union destructor doesn't actually
+        destroy anything because it isn't clear what to destroy (this
+        is dictated by the C++ standard). Instead, the epilog provides
+        a fancy update to destroy things.
+
+        In practice, this means that programs can only destroy unions
+        automatically where they can prove the active entry has a
+        trivial destructor or is already destroyed.
+        *)
+        |={⊤}=> thisp |-> tblockR (Tnamed dtor.(d_class)) (cQp.mut 1) **
+        (
+          thisp |-> tblockR (Tnamed dtor.(d_class)) (cQp.mut 1) -*
+          |={⊤}=> |> Forall p : ptr, p |-> primR Tvoid (cQp.mut 1) Vvoid -* Q p
+        )
+      | _ => None
+      end
+    in
+    match epilog , args with
+    | Some epilog , thisp :: nil =>
+      (**
+      The function consumes a step
+      *)
+      |>
+      let* :=
+        match body return Kpred -> mpred with
+        | Defaulted => fun k => |={top}=> k Normal
+        | UserDefined body => wp tu (Remp (Some thisp) None Tvoid) body
         end
-      | _ => ERROR "constructor without leading [this] argument"
-      end
-    end%I%bs.
-
-  Definition ctor_ok (ctor : Ctor) (spec : function_spec)
-    : mpred :=
-    [| type_of_spec spec = type_of_value (Oconstructor ctor) |] **
-    (* forall each argument, apply to [fs_spec] *)
-    □ Forall Q : ptr -> mpred, Forall vals,
-      spec.(fs_spec) vals Q -* wp_ctor ctor vals Q.
-
-  (** ** Weakest precondition of a destructor *)
-  Definition wpd_bases (cls : globname) (this : ptr) (bases : list globname) : epred -> mpred :=
-    let del_base base := FreeTemps.delete (Tnamed base) (this ,, _base cls base) in
-    interp (FreeTemps.seqs_rev (List.map del_base bases)).
-
-  Lemma wpd_bases_frame cls this : forall bases Q Q',
-      Q -* Q' |-- wpd_bases cls this bases Q -* wpd_bases cls this bases Q'.
-  Proof. intros. apply interp_frame. Qed.
-
-  Definition wpd_members (cls : globname) (this : ptr) (members : list Member) : epred -> mpred :=
-    let del_member m := FreeTemps.delete m.(mem_type) (this ,, _field {| f_name := m.(mem_name) ; f_type := cls |}) in
-    interp (FreeTemps.seqs_rev (List.map del_member members)).
-
-  Lemma wpd_members_frame cls this : forall members Q Q',
-      Q -* Q' |-- wpd_members cls this members Q -* wpd_members cls this members Q'.
-  Proof. intros; apply interp_frame. Qed.
-
-  (** [wp_dtor dtor args Q] defines the semantics of the destructor [dtor] when
-      applied to [args] with post-condition [Q].
-
-      Note that destructors are not always syntactically distinguished from
-      function calls (e.g. in the case of [c.~C()]). Therefore, in order to
-      have a uniform specification, they need to return the underlying memory
-      (i.e. a [this |-> tblockR (Tnamed cls) 1]) to the caller.
-      When the program is destroying this object, e.g. due to stack allocation,
-      this resource will be consumed immediately.
-   *)
-  Definition wp_dtor (dtor : Dtor) (args : list ptr)
-             (Q : ptr -> epred) : mpred :=
-    match dtor.(d_body) with
-    | None => False
-    | Some body =>
-      let epilog :=
-          match tu !! dtor.(d_class) with
-          | Some (Gstruct s) => Some $ fun (thisp : ptr) =>
-            thisp |-> structR dtor.(d_class) (cQp.mut 1) **
-            wpd_members dtor.(d_class) thisp s.(s_fields)
-               (* ^ fields are destroyed *)
-               (thisp |-> wp_revert_identity dtor.(d_class)
-               (* ^ the identity of the object is destroyed *)
-                  (wpd_bases dtor.(d_class) thisp (List.map fst s.(s_bases))
-                  (* ^ the base classes are destroyed (reverse order) *)
-                     (thisp |-> tblockR (Tnamed dtor.(d_class)) (cQp.mut 1) -* |={⊤}=> |> Forall p : ptr, p |-> primR Tvoid (cQp.mut 1) Vvoid -* Q p)))
-                     (* ^ the operations above destroy each object returning its memory to
-                        the abstract machine. Then the abstract machine gives this memory
-                        back to the program.
-                        NOTE the [|>] here is for the function epilog.
-                      *)
-          | Some (Gunion u) => Some $ fun (thisp : ptr) =>
-            (* the function epilog of a union destructor doesn't actually destroy anything
-               because it isn't clear what to destroy (this is dictated by the C++ standard).
-               Instead, the epilog provides a fancy update to destroy things.
-
-               In practice, this means that programs can only destroy unions
-               automatically where they can prove the active entry has a trivial destructor
-               or is already destroyed.
-             *)
-            |={⊤}=> thisp |-> tblockR (Tnamed dtor.(d_class)) (cQp.mut 1) **
-                   (thisp |-> tblockR (Tnamed dtor.(d_class)) (cQp.mut 1) -* |={⊤}=> |> Forall p : ptr, p |-> primR Tvoid (cQp.mut 1) Vvoid -* Q p)
-          | _ => None
-          end%I
       in
-      match epilog , args with
-      | Some epilog , thisp :: nil =>
-        let ρ := Remp (Some thisp) None Tvoid in
-          |> (* the function prolog consumes a step. *)
-             match body return Kpred -> mpred with
-             | Defaulted => fun k => |={top}=> k Normal
-             | UserDefined body => wp ρ body
-             end (Kreturn_void (epilog thisp))
-      | _ , _ => False
-      end
-    end%bs%I.
+      Kreturn_void (epilog thisp)
+    | None , _ => ERROR "wp_dtor: not a structure or union"
+    | Some _ , _ => ERROR "wp_dtor: expected one argument"
+    end
+  end%I.
 
 (*
-  template<typename T>
-  struct optional {
-    union U { T val; char nothing[sizeof(T)]; ~u() {} } u;
-    bool has_value;
-    ~optional() {
-      if (has_value)
-        val.~T();
+template<typename T>
+struct optional {
+  union U { T val; char nothing[sizeof(T)]; ~u() {} } u;
+  bool has_value;
+  ~optional() {
+    if (has_value)
+      val.~T();
 
-    } // has_value.~bool(); u.~U();
-  }
+  } // has_value.~bool(); u.~U();
+}
 
-  p |-> classR .... -* |==> p |-> tblockR "class" 1
+p |-> classR .... -* |==> p |-> tblockR "class" 1
 
-  union { int x; short y; } u;
-    // u |-> tblockR "U" 1
-    // CREATE(0)
-    u.x = 1;
-    // DESTROY(0)
-    // CREATE(1)
-    u.y = 1;
-    // DESTROY(1)
-    // u |-> tblockR "U" 1
+union { int x; short y; } u;
+  // u |-> tblockR "U" 1
+  // CREATE(0)
+  u.x = 1;
+  // DESTROY(0)
+  // CREATE(1)
+  u.y = 1;
+  // DESTROY(1)
+  // u |-> tblockR "U" 1
 
-    // [CREATE(n)] implicit pick a union branch
-    u |-> tblockR "U" 1 ==*
-        u |-> (upaddingR "U" 1 ** ucaseR "U" 0 1 ** _field "x" |-> uninitR "U" 1)
-    // [DESTROY(n)] implicit "destruction" of the union
-    u |-> (upaddingR "U" 1 ** ucaseR "U" 0 1 ** _field "x" |-> uninitR "U" 1) ==*
-        u |-> tblockR "U" 1
+  // [CREATE(n)] implicit pick a union branch
+  u |-> tblockR "U" 1 ==*
+      u |-> (upaddingR "U" 1 ** ucaseR "U" 0 1 ** _field "x" |-> uninitR "U" 1)
+  // [DESTROY(n)] implicit "destruction" of the union
+  u |-> (upaddingR "U" 1 ** ucaseR "U" 0 1 ** _field "x" |-> uninitR "U" 1) ==*
+      u |-> tblockR "U" 1
 *)
 
-  Definition dtor_ok (dtor : Dtor) (spec : function_spec)
-    : mpred :=
-    [| type_of_spec spec = type_of_value (Odestructor dtor) |] **
-    □ Forall Q : ptr -> mpred, Forall vals,
-      spec.(fs_spec) vals Q -* wp_dtor dtor vals Q.
-
-End with_cpp.
-(* conveniences for the common pattern *)
-Notation init_derivationR cls path q := (derivationR cls%bs (path%bs ++ [cls%bs]) q).
-Notation init_derivationsR cls path q := (derivationsR cls%bs (path%bs ++ [cls%bs]) q).
+Definition dtor_ok `{Σ : cpp_logic, σ : genv} (tu : translation_unit)
+    (dtor : Dtor) (spec : function_spec) : mpred :=
+  [| type_of_spec spec = type_of_value (Odestructor dtor) |] **
+  □ Forall (Q : ptr -> mpred) vals,
+  spec.(fs_spec) vals Q -* wp_dtor tu dtor vals Q.
